modélisation Isabelle/HOModel.v
@@ -1,0 +1,139 @@
+Require Import Ensembles.
+Require Import List.
+Require Import ListSet.
+Require Import Coq.Logic.FunctionalExtensionality.
+Require Import Classical.
+
+Parameter msg proc pst: Type.
+Parameter undefined : proc.
+Axiom proc_dec : forall x y:proc, {x = y} + {x <> y}.
+
+Inductive message : Type :=
+  | Content : msg -> message
+  | Void : message
+  | Bot : message.
+
+Inductive proc_state : Type :=
+  | Active : pst -> proc_state
+  | Aslept : proc_state.
+
+Record CHOAlgorith := {
+  CinitState : proc -> pst -> proc -> Prop;
+  SendMsg : proc -> proc -> pst -> msg;
+  CnextState : proc -> pst -> (proc -> message) -> proc -> pst -> Prop }.
+
+Definition initState alg p st : Prop := CinitState alg p st undefined.
+Definition nextState alg p st msgs st' := CnextState alg p st msgs undefined st'.
+
+Definition HO := proc -> Ensemble proc.
+Definition coord := proc -> proc.
+
+Definition SHOmsgVectors A p cfg (HOp:set proc) SHOp :=
+  { mu : proc -> message | (forall q:proc, set_In q HOp <-> mu q <> Void) /\
+      forall q, set_In q (set_inter proc_dec HOp SHOp) -> match cfg q with
+  | Active s => mu q = Content (SendMsg A q p s)
+  | _ => mu q = Bot end}.
+
+Definition CSHOnextConfig A cfg HO SHO coord cfg' : Prop :=
+   forall p, match cfg p with
+  | Active s => match cfg' p with
+    | Active s' => exists mu : (SHOmsgVectors A p cfg (HO p) (SHO p)),
+           CnextState A p s (proj1_sig mu) (coord p) s'
+    | _ => False end
+  | _ => True end.
+
+Definition CHOinitConfig A rho coord :=
+  forall p : proc, exists n : nat, (forall m, m < n -> rho m p = Aslept) /\
+  match rho n p with 
+  |Active s => CinitState A p s (coord n p)
+  | _ => False end.
+
+Definition CSHORun A rho HOs SHOs coords :=
+  CHOinitConfig A rho coords
+   /\ (forall r, CSHOnextConfig A (rho r) (HOs r) (SHOs r) (coords (S r)) (rho (S r))).
+
+Definition HOinitConfig  A cfg := CHOinitConfig A cfg (fun _ _ => undefined).
+
+Lemma HOinitConfig_eq : forall A cfg, HOinitConfig A cfg =
+  forall p:proc, exists n:nat, (forall m, m < n -> cfg m p = Aslept) /\
+  match cfg n p with 
+  |Active s => initState A p s
+  | _ => False end.
+trivial.
+Qed.
+
+Definition SHOnextConfig A cfg HO SHO cfg' :=
+  CSHOnextConfig A cfg HO SHO (fun _ => undefined) cfg'.
+
+Lemma SHOnextConfig_eq : forall A (cfg:proc->proc_state) HO SHO cfg',
+  SHOnextConfig A cfg HO SHO cfg' = 
+    forall p,  match cfg p with
+  | Active s => match cfg' p with
+    | Active s' => exists mu : SHOmsgVectors A p cfg (HO p) (SHO p),
+        nextState A p s (proj1_sig mu) s'
+    | _ => False end
+  | _ => True end.
+trivial.
+Qed.
+
+Definition SHORun A rho HOs SHOs := CSHORun A rho HOs SHOs (fun _ _ => undefined).
+
+Lemma SHORun_eq : forall A rho HOs SHOs, SHORun A rho HOs SHOs =
+  (HOinitConfig A rho /\ (forall r, SHOnextConfig A (rho r) (HOs r) (SHOs r) (rho (S r)))).
+trivial.
+Qed.
+
+Definition HOrcvMsgs A p (HO:set proc) cfg := fun q : proc =>
+  match set_In_dec proc_dec q HO with
+  | left _ => 
+    match cfg q with
+    | Active s =>  Content (SendMsg A q p s)
+    | Aslept => Bot end
+  | right _ => Void end.
+
+Lemma SHOmsgVectors_HO : forall A p cfg HO,
+  forall mu : SHOmsgVectors A p cfg HO HO, proj1_sig mu = HOrcvMsgs A p HO cfg.
+intros.
+apply functional_extensionality.
+intro.
+induction mu.
+unfold proj1_sig.
+unfold HOrcvMsgs.
+case (set_In_dec proc_dec x HO0); intro.
+assert (s2:=s).
+apply p0 in s.
+assert (s3 := (proj2 p0)  x (set_inter_intro proc_dec x HO0 HO0 s2 s2)).
+
+destruct (cfg x).
+assumption.
+assumption.
+
+assert (H:=proj1 p0 x).
+apply not_iff_compat in H.
+apply H in n.
+apply NNPP in n.
+trivial.
+Qed.
+
+Definition CHOnextConfig A cfg HO coord cfg' :=
+   CSHOnextConfig A cfg HO HO coord cfg'.
+
+Lemma CHOnextConfig_eq : forall A cfg HO coord cfg',
+  CHOnextConfig A cfg HO coord cfg' =
+  forall p,  match cfg p with
+  | Active s => match cfg' p with
+    | Active s' => CnextState A p s (HOrcvMsgs A p (HO p) cfg) (coord p) s'
+    | _ => False end
+  | _ => True end.
+intros.
+unfold CHOnextConfig.
+unfold CSHOnextConfig.
+apply forall_extensionalityP.
+intro.
+case (cfg x).
+intro.
+case (cfg' x).
+intro.
+unfold HOrcvMsgs.
+rewrite <- (SHOmsgVectors_HO.
+trivial.
